Working on free var names stuff
Part of proof about alpha conversion with nodup free vars
(true in general but hard to prove)
Proof that, assuming this, conversion satisfies strong
wf
Need to prove that strong wf implies recursive wf

proofs/core/Theory.v
@@ -2249,53 +2249,6 @@ Definition tm_wf_strong_rec := P_subtm
 Definition fmla_wf_strong_rec := P_subfmla
 (fun _ => True) tm_wf_strong fmla_wf_strong.
 
-(*Plan
-  1. Prove if Nodup names of bnd, then NoDup names of bnd for all subterms/fmlas
-  2. Prove that all bnd in subterms/fmlas are in t
-  3. Use the above (plus fv lemma) to show that
-    no overlap in subterms (or else overlap in t)
-  4. Prove that if strong condition holds, no free variable dups in any
-    subterm
-  5. put together (no induction)
-  *)
-
-(*Want to show: if we have a term satisfying this condition,
-  then it satisfies it recursively*)
-  (*
-Lemma wf_strong_rec_holds t f:
-  (forall (Hwf: tm_wf_strong t), tm_wf_strong_rec t) /\
-  (forall (Hwf: fmla_wf_strong f), fmla_wf_strong_rec f).
-Proof.
-  unfold tm_wf_strong_rec, fmla_wf_strong_rec.
-  rewrite -> P_subterms_equiv, P_subfmlas_equiv. split.
-  - intros. split_all; auto. 3: rewrite Forall_forall; auto.
-    + unfold tm_wf_strong in *.
-      destruct_all.
-
-  
-  split; intros. unfold tm_wf_strong;
-  revert t f. unfold tm_wf_strong_rec, fmla_wf_strong_rec. 
-  apply term_formula_ind; simpl; intros.
-  - cbn. split; auto.
-  - cbn. split; auto.
-  - cbn. split; auto.
-    simpl_forall.
-    revert H. apply Forall_impl_in.
-    intros. apply H0.
-    clear -Hwf H.
-    unfold tm_wf_strong in *.
-    simpl in *. split_all.
-    + induction l1; simpl in *; try contradiction.
-      destruct H; subst.
-      * erewrite -> map_union  with(eq_dec2:=string_dec) in H0.
-
-
-    
-    rewrite Forall_forall; intros.
-    
-    simpl.
-
-*)
 
 (*Now prove that if a term has no duplicate bound variable
   names and is closed, then *)
@@ -3538,7 +3491,836 @@ Proof.
     generalize dependent (v_subst (vt_with_args vt params (map (v_subst vt) tys)) ty1); intros; subst; 
     unfold dom_cast; simpl.
     reflexivity.
-  - 
+  - (*Fpred*)
+    assert (Hmap: (map (v_subst vt) (ty_subst_list' params tys tys0)) =
+    (map (v_subst (vt_with_args vt params (map (v_subst vt) tys))) tys0)). {
+      apply list_eq_ext'; rewrite !map_length; auto.
+      intros n d Hn. unfold ty_subst_list'.
+      rewrite !map_map.
+      rewrite -> !map_nth_inbound with (d2:=vty_int); auto.
+      apply v_subst_vt_with_args'.
+    }
+    assert (Hargs:
+    cast_arg_list (f_equal (sym_sigma_args p) Hmap)
+    (pred_arg_list pd vt p (ty_subst_list' params tys tys0) (map ty_subst_tm tms)
+    (term_rep gamma_valid pd vt pf vv1) Hty2) =
+    (pred_arg_list pd (vt_with_args vt params (map (v_subst vt) tys)) p tys0 tms
+        (term_rep gamma_valid pd (vt_with_args vt params (map (v_subst vt) tys)) pf
+          vv2) Hty1)).
+    {
+      unfold pred_arg_list.
+      apply (get_arg_list_vt_ext') with(s:=p)(Heq:=Hmap);
+      rewrite map_length; auto.
+      revert H; rewrite Forall_forall; intros.
+      revert Hty0. rewrite -> map_nth_inbound with (d2:=tm_d); auto.
+      intros.
+      erewrite H; [|apply nth_In; auto | |].
+      rewrite !dom_cast_compose. apply dom_cast_refl.
+      cbn in Hwf; destruct_all.
+      simpl_forall. rewrite Forall_forall in H2; apply H2; apply nth_In; auto.
+      intros. apply Hvv. simpl_set.
+      exists (nth i tms tm_d); split; auto; apply nth_In; auto.
+      Unshelve.
+      auto.
+    }
+    rewrite <- Hargs.
+    rewrite <- preds_cast_eq. reflexivity.
+  - (*Fquant*)
+    assert (Heq: v_subst vt (ty_subst_var v).2 =
+    v_subst (vt_with_args vt params (map (v_subst vt) tys)) v.2).
+    {
+      simpl. apply v_subst_vt_with_args'.
+    }
+    assert (forall d1 d2,
+      d1 = dom_cast (dom_aux pd) Heq d2 ->
+      formula_rep gamma_valid pd vt pf (substi pd vt vv1 (ty_subst_var v) d2) 
+      (ty_subst_fmla f) (typed_quant_inv Hty2) =
+    formula_rep gamma_valid pd (vt_with_args vt params (map (v_subst vt) tys)) pf
+      (substi pd (vt_with_args vt params (map (v_subst vt) tys)) vv2 v d1) f
+      (typed_quant_inv Hty1)).
+    {
+      intros. subst. apply H; auto. apply Hwf.
+      intros. unfold substi.
+      vsym_eq x v.
+      - vsym_eq (ty_subst_var v) (ty_subst_var v). simpl.
+        assert (e = Logic.eq_refl) by (apply UIP_dec; apply vsymbol_eq_dec); subst.
+        apply dom_cast_eq.
+      - vsym_eq (ty_subst_var x) (ty_subst_var v); [| apply Hvv; simpl_set; auto].
+        exfalso. destruct Hwf as [Hwf _].
+        unfold fmla_wf_strong in Hwf.
+        destruct Hwf as [_ [_ Hwf]].
+        apply ty_subst_var_fst in e.
+        apply (Hwf (fst x)); split; rewrite in_map_iff; simpl;
+        [exists x | exists v]; simpl_set; auto.
+    }
+    destruct q; simpl_rep_full;
+    apply all_dec_eq; split; intros.
+    + erewrite <- H0. apply H1.
+      Unshelve.
+      2: exact (dom_cast (dom_aux pd) (Logic.eq_sym Heq) d).
+      rewrite !dom_cast_compose. symmetry. apply dom_cast_refl.
+    + erewrite H0. apply H1. reflexivity.
+    + destruct H1 as [d Hd]. exists (dom_cast (dom_aux pd) Heq d).
+      erewrite <- H0. apply Hd. reflexivity.
+    + destruct H1 as [d Hd]. exists (dom_cast (dom_aux pd) (Logic.eq_sym Heq) d).
+      erewrite H0. apply Hd. rewrite !dom_cast_compose. symmetry.
+      apply dom_cast_refl.
+  - (*Feq*)
+    apply all_dec_eq. 
+    assert (Heq1: v_subst (vt_with_args vt params (map (v_subst vt) tys)) v =
+    v_subst vt (ty_subst' params tys v)).
+    {
+      symmetry.
+      apply v_subst_vt_with_args'.
+    }
+    rewrite -> H with(vv2:=vv2)(ty1:=v)(Hty1:=proj1' (typed_eq_inv Hty1))(Heq:=Heq1);
+    [| apply Hwf | intros; apply Hvv; simpl_set; auto].
+    rewrite -> H0 with(vv2:=vv2)(ty1:=v)(Hty1:=proj2' (typed_eq_inv Hty1))(Heq:=Heq1);
+    [| apply Hwf | intros; apply Hvv; simpl_set; auto].
+    split; intros Heq.
+    + apply dom_cast_inj in Heq. auto.
+    + rewrite Heq. apply dom_cast_eq.
+  - (*Fbinop - easier bc no casts*)
+    rewrite -> H with(vv2:=vv2)(Hty1:=proj1' (typed_binop_inv Hty1));
+    [|apply Hwf | intros; apply Hvv; simpl_set; auto].
+    rewrite -> H0 with (vv2:=vv2)(Hty1:=proj2' (typed_binop_inv Hty1));
+    [|apply Hwf | intros; apply Hvv; simpl_set; auto].
+    reflexivity.
+  - (*Fnot*)
+    rewrite -> H with (vv2:=vv2)(Hty1:=typed_not_inv Hty1); auto.
+    apply Hwf.
+  - (*Flet*)
+    assert (Heq1: v_subst (vt_with_args vt params (map (v_subst vt) tys)) v.2 =
+    v_subst vt (ty_subst' params tys v.2)).
+    {
+      symmetry; apply v_subst_vt_with_args'.
+    }
+    (*cbn in Hwf. destruct_all.*)
+    rewrite -> H with(vv2:=vv2)(ty1:=snd v)(Heq:=Heq1)(Hty1:=(proj1' (typed_let_inv Hty1))); auto;
+    [|apply Hwf | intros; apply Hvv; simpl_set; auto].
+    apply H0; [apply Hwf |].
+    intros.
+    (*separate lemma?*)
+    unfold substi.
+    vsym_eq x v.
+    + vsym_eq (ty_subst_var v) (ty_subst_var v).
+      simpl. assert (e = Logic.eq_refl) by (apply UIP_dec; apply vsymbol_eq_dec);
+      subst; simpl. rewrite dom_cast_compose. symmetry. apply dom_cast_refl.
+    + vsym_eq (ty_subst_var x) (ty_subst_var v); 
+      [| apply Hvv; intros; simpl_set; auto].
+      exfalso. destruct Hwf as [Hwf _].
+      destruct Hwf as [_ [_ Hwf]].
+      apply (Hwf (fst x)).
+      apply ty_subst_var_fst in e.
+      split; rewrite in_map_iff; simpl; [exists x | exists v];
+      simpl_set; auto.
+  - (*Fif*)
+    rewrite -> H with (vv2:=vv2)(Hty1:=proj1' (typed_if_inv Hty1));
+    [| apply Hwf | intros; apply Hvv; simpl_set; auto].
+    rewrite -> H0 with (vv2:=vv2)(Hty1:=proj1' (proj2' (typed_if_inv Hty1)));
+    [| apply Hwf | intros; apply Hvv; simpl_set; auto].
+    rewrite -> H1 with (vv2:=vv2)(Hty1:=proj2' (proj2' (typed_if_inv Hty1)));
+    [| apply Hwf | intros; apply Hvv; simpl_set; auto].
+    reflexivity.
+  -(*Fmatch*)
+    iter_match_gen Hty1 Htm1 Hpat1 Hty1.
+    iter_match_gen Hty2 Htm2 Hpat2 Hty2.
+    cbn in Hwf. destruct Hwf as [Hwf [Hptm Hpall]].
+    (*From Hwf, get info we need about bnd and free vars*)
+    assert (Hbndfree: forall p f x y,
+      In (p, f) ps ->
+      In x (pat_fv p) ->
+      In y (fmla_fv f) ->
+      fst x = fst y ->
+      x = y).
+    {
+      intros p f x y Hinpt Hinx Hiny Hxy. 
+      unfold fmla_wf_strong in Hwf; simpl in Hwf.
+      vsym_eq x y.
+      destruct (in_dec vsymbol_eq_dec y (pat_fv p)).
+      {
+        destruct Hwf as [_ [Hwf _]].
+        revert Hwf.
+        rewrite -> map_app, NoDup_app_iff.
+        intros [_ [Hwf _]].
+        eapply NoDup_map_in. apply Hwf. all: auto;
+        rewrite in_concat; eexists;
+        split; try (rewrite in_map_iff);
+        try (eexists; split; [reflexivity | auto]);
+        try apply Hinpt;
+        rewrite !in_app_iff; auto.
+      }
+      (*Now y not in, so can use 3rd part of Hwf*)
+      destruct Hwf as [_ [_ Hwf]].
+      exfalso.
+      apply (Hwf (fst x)).
+      rewrite map_app. split.
+      - rewrite !in_map_iff. exists y.
+        split; auto. simpl_set. right. exists (p, f); split; auto.
+        simpl_set; auto.
+      - rewrite in_app_iff. right.
+        rewrite in_map_iff. exists x. split; auto.
+        rewrite in_concat. eexists.
+        split. rewrite in_map_iff. eexists; split; [reflexivity | auto].
+        apply Hinpt. rewrite in_app_iff; auto.
+    }
+    clear Hwf. rewrite Forall_map in Hpall.
+    induction ps; simpl; intros; auto.
+    destruct a.
+    inversion H0; subst.
+    (*First step: handle term_rep in case*)
+    assert (Heq1: v_subst (vt_with_args vt params (map (v_subst vt) tys)) v =
+    v_subst vt (ty_subst' params tys v)).
+    {
+      symmetry; apply v_subst_vt_with_args'.
+    }
+    erewrite -> H with(vv2:=vv2)(ty1:=v)(Hty1:=Hty1)(Heq:=Heq1);
+    auto.
+    2: { intros; rewrite Hvv; auto; simpl_set; auto. }
+    simpl.
+    case_match_goal.
+    2: {
+      (*TODO: naming*)
+      rewrite -> match_val_single_vt_none in Hmatch.
+      rewrite -> Hmatch.
+      rewrite <- H with(vv1:=vv1)(Hty2:=Hty2). auto. simpl. 
+      apply IHps. all: auto.
+      - intros. apply Hvv. simpl; simpl_set_small; auto.
+        destruct H1; auto.
+      - intros. apply (Hbndfree p0 f0 x y); simpl; auto.  
+      - inversion Hpall; subst; auto.
+      - intros. apply Hvv. simpl; simpl_set_small; auto.
+    }
+    symmetry.
+    destruct (match_val_single gamma_valid pd (vt_with_args vt params (map (v_subst vt) tys)) v p
+    (Forall_inv Hpat1)
+    (term_rep gamma_valid pd (vt_with_args vt params (map (v_subst vt) tys)) pf vv2
+      tm v Hty1)) eqn : Hmatch1.
+    2: {
+      rewrite <- match_val_single_vt_none in Hmatch1.
+      rewrite -> Hmatch1 in Hmatch. inversion Hmatch.
+      (*Contradiction from [match_val_single_vt_none]*)
+    }
+    symmetry.
+    apply H3.
+    { apply (Forall_inv Hpall). }
+    intros x Hinx Heq'.
+    destruct (in_dec vsymbol_eq_dec x (pat_fv p)).
+    2: {
+      (*Not in: follows from Hvv*)
+      rewrite !extend_val_notin; auto.
+      - erewrite Hvv. reflexivity.
+        simpl. simpl_set; auto.
+      - rewrite <- (match_val_single_free_var gamma_valid pd vt). 
+        2: apply Hmatch.
+        rewrite ty_subst_p_fv.
+        rewrite in_map_iff.
+        intros C. destruct C as [y [Hxy Hiny]].
+        (*Contradicts fact that no names shared between bnd and free vars*)
+        assert (x = y). {
+          symmetry.
+          apply (Hbndfree p f y x); simpl; auto.
+          apply ty_subst_var_fst in Hxy; auto.
+        }
+        subst. contradiction.
+      - rewrite <- (match_val_single_free_var gamma_valid pd 
+        (vt_with_args vt params (map (v_subst vt) tys))).
+        2: apply Hmatch1. apply n.
+    }
+    (*So now we know that x is in (pat_fv p), and
+      therefore we know that it is in (map fst l0)*)
+    assert (In x (map fst l0)). {
+      rewrite <- (match_val_single_free_var gamma_valid pd 
+        (vt_with_args vt params (map (v_subst vt) tys))).
+      apply i. apply Hmatch1.
+    }
+    rewrite in_map_iff in H1.
+    destruct H1 as [[x1 y1] [Hx Hinx1]]; subst; simpl in *.
+    rewrite -> extend_val_lookup with (t:=y1); auto.
+    2:  apply match_val_single_nodup in Hmatch1; auto.
+    (*TODO: see what we need for other*)
+    assert (projT1 y1 = (v_subst (vt_with_args vt params (map (v_subst vt) tys)) x1.2)).
+    {
+      eapply match_val_single_typs. apply Hmatch1. auto.
+    }
+    destruct (sort_eq_dec (v_subst (vt_with_args vt params (map (v_subst vt) tys)) x1.2) (projT1 y1));
+    try (exfalso; apply n; auto).
+    assert (exists z Heq,
+      In (ty_subst_var x1, z) l /\
+      projT2 z = dom_cast (dom_aux pd) Heq (projT2 y1)
+    ).
+    { eapply match_val_single_vt_some. apply Hmatch. 
+      apply Hmatch1. auto. }
+    destruct H2 as [z [Hz1 [Hinz Hz2]]].
+    rewrite -> extend_val_lookup with (t:=z); auto.
+    2: apply match_val_single_nodup in Hmatch; auto.
+    assert (projT1 z = (v_subst vt (ty_subst_var x1).2)). {
+      rewrite <- Hz1, <- e. symmetry.
+      apply v_subst_vt_with_args'.
+    }
+    destruct (sort_eq_dec (v_subst vt (ty_subst_var x1).2) (projT1 z));
+    [| exfalso; apply n; auto].
+    rewrite Hz2. rewrite !dom_cast_compose. apply dom_cast_eq.
+Qed.
+
+Definition ty_subst_t_rep {pd} t (pf: pi_funpred gamma_valid pd) := 
+    proj_tm (@ty_subst_tf_rep pd pf) t.
+Definition ty_subst_f_rep {pd} f (pf: pi_funpred gamma_valid pd) := 
+  proj_fmla (@ty_subst_tf_rep pd pf) f.
+
+(*Now we need to relax the assumptions.
+  The first step is to prove that tm_wf_strong implies tm_wf_strong_rec.
+  In other words, the recursive part adds nothing
+  (but it makes the above proofs much easier) *)
+
+
+  (*Is this true?*)
+(*This lemma boils down to lots of case analysis in
+  the "interesting" cases (with bound vars) - the tactics
+  above automate this pretty well*)
+
+  (*Don't think shape hyp is really needed but *)
+
+(*Maybe alternate approach: if alpha-equivalent accoridng to vars,
+  then tm_fv t1 = map (lookup_fv vars) (tm_fv t2) *)
+Definition lookup_fv (vars: list (vsymbol * vsymbol)) (x: vsymbol) : vsymbol :=
+  match (get_assoc_list vsymbol_eq_dec vars x) with
+  | Some y => y
+  | _ => x
+  end.
+
+Lemma eq_vars_lookup vars x y:
+  eq_var vars x y ->
+  lookup_fv vars x = y.
+Proof.
+  unfold lookup_fv. intros.
+  destruct (get_assoc_list vsymbol_eq_dec vars x) eqn : Ha.
+  - induction vars; simpl in *; try discriminate.
+    vsym_eq x (fst a); simpl in *.
+    + inversion Ha; subst.
+      vsym_eq y (snd a). inversion H.
+    + vsym_eq y (snd a).
+  - apply get_assoc_list_none in Ha.
+    rewrite eq_var_eq in H.
+    destruct (in_firstb vsymbol_eq_dec vsymbol_eq_dec (x, y) vars) eqn : Hinb.
+    { apply in_firstb_in in Hinb. exfalso. apply Ha. rewrite in_map_iff.
+      exists (x, y); auto. }
+    simpl in H.
+    vsym_eq x y.
+    simpl in H. revert H; simpl_bool; discriminate.
+Qed.
+Print a_convert_all_t.
+Print alpha_t_aux.
+
+Search NoDup map union.
+
+(*Another recursive condition: no free or bound variable names appear
+  in list l*)
+
+Lemma remove_nodup {A} (eq_dec: forall (x y: A), {x = y} + {x <> y}) x l:
+  NoDup l ->
+  NoDup (remove eq_dec x l).
+Proof.
+  intros. induction l; simpl; auto.
+  inversion H; subst.
+  destruct (eq_dec x a); auto. constructor; auto.
+  simpl_set. intros [Hina Hax].
+  contradiction.
+Qed.
+
+Lemma fv_nodup t f:
+  NoDup (tm_fv t) /\ NoDup (fmla_fv f).
+Proof.
+  revert t f; apply term_formula_ind; simpl; intros;
+  try solve[repeat(constructor; auto)];
+  repeat (apply big_union_nodup +
+  apply union_nodup + apply remove_nodup); auto.
+Qed.
+
+Definition tm_fv_nodup t := proj_tm fv_nodup t.
+Definition fmla_fv_nodup f := proj_fmla fv_nodup f.
+
+(*copied: TODO*)
+(**Disjoint lists*)
+Section Disj.
+Context {A: Type}.
+Definition disj (l1 l2: list A) : Prop :=
+  forall x, ~ (In x l1 /\ In x l2).
+Lemma disj_l12_iff (l1 l2: list A):
+  disj l1 l2 <-> (forall x, In x l1 -> ~ In x l2).
+Proof.
+  unfold disj.
+  split; intros.
+  - intro C. apply (H _ (conj H0 C)).
+  - intro C. destruct C.
+    apply (H _ H0 H1).
+Qed.
+
+Lemma disj_l12 {l1 l2: list A}:
+  disj l1 l2 -> (forall x, In x l1 -> ~ In x l2).
+Proof.
+  apply disj_l12_iff.
+Qed.
+
+Lemma disj_comm (l1 l2: list A):
+  disj l1 l2 <-> disj l2 l1.
+Proof.
+  unfold disj. split; intros; rewrite and_comm; auto.
+Qed.
+
+Lemma disj_l21_iff (l1 l2: list A):
+  disj l1 l2 <-> (forall x, In x l2 -> ~ In x l1).
+Proof.
+  rewrite disj_comm. apply disj_l12_iff.
+Qed.
+
+Lemma disj_l21 {l1 l2: list A}:
+  disj l1 l2 -> (forall x, In x l2 -> ~ In x l1).
+Proof.
+  apply disj_l21_iff.
+Qed.
+
+Lemma disj_sublist {l1 l2 l3: list A}:
+  disj l1 l2 ->
+  sublist l3 l2 ->
+  disj l1 l3.
+Proof.
+  unfold disj, sublist; intros Hsub Hdisj x [Hinx1 Hinx2].
+  apply (Hsub x); split; auto.
+Qed.
+
+End Disj.
+
+(*Other results about disj*)
+
+Lemma split_lens_disj {A: Type} (l1: list A) l2 lens i:
+  disj l1 l2 ->
+  sum lens = length l1 ->
+  disj (nth i (split_lens l1 lens) nil) l2.
+Proof.
+  unfold disj. intros.
+  intros [Hinx1 Hinx2].
+  assert ((i < length lens)%coq_nat \/ (i >= length lens)%coq_nat) by lia.
+  destruct H1.
+  - apply in_split_lens_ith in Hinx1; wf_tac.
+    apply (H x); auto.
+  - rewrite nth_overflow in Hinx1; try contradiction.
+    rewrite split_lens_length. lia.
+Qed.
+
+Lemma firstn_disj {A: Type} (l1 l2: list A) n:
+  disj l1 l2 ->
+  disj (firstn n l1) l2.
+Proof.
+  intros. unfold disj in *. intros.
+  intros [Hinx1 Hinx2].
+  apply In_firstn in Hinx1.
+  apply (H x); auto.
+Qed.
+
+Lemma skipn_disj {A: Type} (l1 l2: list A) n:
+  disj l1 l2 ->
+  disj (skipn n l1) l2.
+Proof.
+  intros. unfold disj in *. intros.
+  intros [Hinx1 Hinx2].
+  apply In_skipn in Hinx1.
+  apply (H x); auto.
+Qed.
+
+Lemma sublist_map {A B: Type} (f: A -> B) (l1 l2: list A):
+  sublist l1 l2 ->
+  sublist (map f l1) (map f l2).
+Proof.
+  apply incl_map.
+Qed.
+
+Lemma sublist_big_union {A B: Type} (eq_dec: forall x y: A, {x = y} + {x <> y})
+(f: B -> list A) (l: list B)
+(x: B):
+In x l ->
+sublist (f x) (big_union eq_dec f l).
+Proof.
+  intros. unfold sublist. intros.
+  simpl_set. exists x; auto.
+Qed.
+
+Lemma sublist_concat_map {A B: Type} (f: A -> list B) x (l: list A):
+  In x l ->
+  sublist (f x) (concat (map f l)).
+Proof.
+  intros. unfold sublist. intros.
+  rewrite in_concat. exists (f x); split; auto.
+  rewrite in_map_iff. exists x; auto.
+Qed.
+
+Lemma nodup_map_union {A B : Type} (eq_dec1 : forall x y : A, {x = y} + {x <> y})
+(eq_dec2 : forall x y : B, {x = y} + {x <> y})
+(f : A -> B) (l1 l2 : seq.seq A):
+NoDup (map f l1) ->
+NoDup (map f l2) ->
+disj (map f l1) (map f l2) ->
+NoDup (map f (union eq_dec1 l1 l2)).
+Proof.
+  intros. rewrite -> map_union with(eq_dec2:=eq_dec2).
+  - apply union_nodup; auto.
+  - intros x y. rewrite !in_app_iff; intros; destruct_all; subst; auto.
+    + eapply NoDup_map_in. apply H. all: auto.
+    + exfalso. apply (H1 (f x)).
+      split; rewrite in_map_iff; [exists y | exists x]; auto.
+    + exfalso. apply (H1 (f x)).
+      split; rewrite in_map_iff; [exists x | exists y]; auto.
+    + eapply NoDup_map_in. apply H0. all: auto.
+Qed.
+
+Lemma nodup_map_union_alt {A B : Type} (eq_dec1 : forall x y : A, {x = y} + {x <> y})
+(eq_dec2 : forall x y : B, {x = y} + {x <> y})
+(f : A -> B) (l1 l2 : seq.seq A):
+NoDup (map f l1) ->
+NoDup (map f l2) ->
+(forall x y, In x l1 -> In y l2 -> f x = f y -> x = y) ->
+NoDup (map f (union eq_dec1 l1 l2)).
+Proof.
+  intros. rewrite -> map_union with(eq_dec2:=eq_dec2).
+  - apply union_nodup; auto.
+  - intros x y. rewrite !in_app_iff; intros; destruct_all; subst; auto.
+    + eapply NoDup_map_in. apply H. all: auto.
+    + symmetry; apply H1; auto.
+    + eapply NoDup_map_in. apply H0. all: auto.
+Qed.
+
+Lemma nodup_map_big_union {A B C: Type} (eq_dec : forall x y : B, {x = y} + {x <> y})
+(eq_dec2: forall x y: C, {x = y} + {x <> y})
+(f : B -> C) (g : A -> seq.seq B) (l : seq.seq A):
+(forall x: A, In x l -> NoDup (map f (g x))) ->
+(forall i j d,
+  (i < length l)%coq_nat -> (j < length l)%coq_nat ->
+  i <> j -> disj (map f (g (nth i l d))) (map f (g (nth j l d)))) ->
+  NoDup (map f (big_union eq_dec g l)).
+Proof.
+  intros. induction l; simpl; try constructor. simpl in *.
+  apply nodup_map_union; auto.
+  - apply IHl; auto.
+    intros. apply (H0 (S i) (S j) d); lia.
+  - intros x [Hinx1 Hinx2].
+    rewrite in_map_iff in Hinx2.
+    destruct Hinx2 as [y [Hx Hiny]]; subst.
+    simpl_set. destruct Hiny as [z [Hinz Hiny]].
+    destruct (In_nth _ _ z Hinz) as [j [Hj Hz]]; subst.
+    rewrite <- Hz in Hinz, Hiny. clear Hz.
+    apply (H0 0 (S j) z ltac:(lia) ltac:(lia) ltac:(lia) (f y)); auto; try lia.
+    split; auto.
+    rewrite in_map_iff. exists y; auto.
+Qed.
+
+Lemma nodup_map_big_union_alt {A B C: Type} (eq_dec : forall x y : B, {x = y} + {x <> y})
+(eq_dec2: forall x y: C, {x = y} + {x <> y})
+(f : B -> C) (g : A -> seq.seq B) (l : seq.seq A):
+(forall x: A, In x l -> NoDup (map f (g x))) ->
+(forall x y l1 l2, In l1 l -> In l2 l ->
+  In x (g l1) -> In y (g l2) -> f x = f y -> x = y) ->
+(*(forall i j d,
+  (i < length l)%coq_nat -> (j < length l)%coq_nat ->
+  i <> j -> disj (map f (g (nth i l d))) (map f (g (nth j l d)))) ->*)
+  NoDup (map f (big_union eq_dec g l)).
+Proof.
+  intros. induction l; simpl; try constructor. simpl in *.
+  apply nodup_map_union_alt; auto.
+  - apply IHl; auto.
+    intros. eapply (H0 _ _ l1 l2); auto.
+  - intros. simpl_set.
+    destruct H2 as [z [Hinz Hiny]].
+    apply (H0 x y a z); auto.
+Qed.
+ (*   
+    intros x [Hinx1 Hinx2].
+    rewrite in_map_iff in Hinx2.
+    destruct Hinx2 as [y [Hx Hiny]]; subst.
+    simpl_set. destruct Hiny as [z [Hinz Hiny]].
+    destruct (In_nth _ _ z Hinz) as [j [Hj Hz]]; subst.
+    rewrite <- Hz in Hinz, Hiny. clear Hz.
+    apply (H0 0 (S j) z ltac:(lia) ltac:(lia) ltac:(lia) (f y)); auto; try lia.
+    split; auto.
+    rewrite in_map_iff. exists y; auto.
+Qed.*)
+
+
+Lemma nodup_map_union_inv_alt {A B: Type} (eq_dec: forall (x y: A), {x = y} + {x <> y})
+  (f: A -> B) (l1 l2: list A):
+  NoDup l1 ->
+  NoDup l2 ->
+  NoDup (map f (union eq_dec l1 l2)) ->
+  (forall x y, In x l1 -> In y l2 -> f x = f y -> x = y).
+Proof.
+  intros.
+  eapply NoDup_map_in. apply H1. all: simpl_set; auto.
+Qed.
+
+Lemma nodup_map_big_union_inv_alt {A B C: Type} (eq_dec: forall (x y: B), {x = y} + {x <> y})
+(f: B -> C) (g: A -> list B) (l: list A)
+(Hg: forall x, In x l -> NoDup (g x)):
+NoDup (map f (big_union eq_dec g l)) ->
+(forall x y l1 l2, In l1 l -> In l2 l ->
+  In x (g l1) -> In y (g l2) -> f x = f y -> x = y).
+Proof.
+  intros.
+  eapply NoDup_map_in. apply H.
+  all: simpl_set; auto.
+  exists l1; auto. exists l2; auto.
+Qed.
+
+Lemma alpha_t_aux_fv t l:
+  NoDup l ->
+  length l = length (tm_bnd t) ->
+  disj l (map fst (tm_fv t)) ->
+  disj l (map fst (tm_bnd t)) ->
+  forall x, In x (tm_fv (alpha_t_aux t l)) <-> In x (tm_fv t).
+Proof.
+  intros. rewrite <- alpha_equiv_t_fv. reflexivity.
+  apply alpha_t_aux_equiv; auto.
+  - intros. intros Hinx.
+    specialize (H1 (fst x0)).
+    apply H1. split; auto. rewrite in_map_iff.
+    exists x0; auto.
+  - intros.
+    specialize (H2 (fst x0)).
+    intro C. apply H2. split; auto. rewrite in_map_iff.
+    exists x0; auto.
+Qed.
+
+
+(*Lemma alpha_t_aux_equiv' t l:
+  NoDup l ->
+  length l = length (tm_bnd t) ->
+  disj l (map fst (tm_fv t)) ->
+  disj l (map fst (tm_bnd t)) ->
+  a_equiv_t t (alpha_t_aux t l).
+Proof.
+  intros. apply alpha_t_aux_equiv; auto.
+  - intros.
+    specialize (H1 (fst x)).
+    intro C.
+    apply H1. split; auto. rewrite in_map_iff.
+    exists x; auto.
+  - intros.
+    specialize (H2 (fst x)).
+    intro C. apply H2. split; auto. rewrite in_map_iff.
+    exists x; auto.
+Qed.*)
+
+Lemma disj_cons_inv {A: Type} {x: A} {l1 l2}:
+  disj (x :: l1) l2 ->
+  disj l1 l2.
+Proof.
+  unfold disj; intros.
+  intros [Hinx1 Hinx2].
+  apply (H x0); simpl; auto.
+Qed.
+
+Lemma union_sublist_l {A: Type} eq_dec (l1 l2: list A):
+  sublist l1 (union eq_dec l1 l2).
+Proof.
+  intros x. simpl_set. intros; auto.
+Qed.
+
+Lemma sublist_app_l {A: Type} (l1 l2: list A):
+  sublist l1 (l1 ++ l2).
+Proof.
+  intros x. rewrite in_app_iff. intros; auto.
+Qed.
+
+Lemma sublist_app_r {A: Type} (l1 l2: list A):
+  sublist l2 (l1 ++ l2).
+Proof.
+  intros x. rewrite in_app_iff. intros; auto.
+Qed.
+
+Lemma map_remove {A B: Type} eq_dec eq_dec2 (f: A -> B) (x: A) (l: list A)
+  (Hinj: forall y z, (y = x \/ In y l) -> (z = x \/ In z l) -> 
+    f y = f z -> y = z):
+  map f (remove eq_dec x l) = remove eq_dec2 (f x) (map f l).
+Proof.
+  induction l; simpl; auto. simpl in *.
+  destruct (eq_dec x a); subst.
+  - destruct (eq_dec2 (f a) (f a)); auto.
+    apply IHl; intros. destruct_all; apply Hinj; auto.
+    contradiction.
+  - destruct (eq_dec2 (f x) (f a)); simpl.
+    + exfalso. apply n. apply Hinj; auto.
+    + f_equal. apply IHl. intros; destruct_all; apply Hinj; auto.
+Qed.
+
+Lemma alpha_aux_fv_NoDup  t f:
+  (forall (l: list string) (Hl: NoDup l) (Hlen: length l = length (tm_bnd t)) 
+    (Hfv: disj l (map fst (tm_fv t)))
+    (Hbnd: disj l (map fst (tm_bnd t)))
+    (Ht: NoDup (map fst (tm_fv t))),
+    NoDup (map fst (tm_fv (alpha_t_aux t l)))
+  ) /\
+  (forall (l: list string) (Hl: NoDup l) (Hlen: length l = length (fmla_bnd f)) 
+    (Hfv: disj l (map fst (fmla_fv f)))
+    (Hbnd: disj l (map fst (fmla_bnd f)))
+    (Ht: NoDup (map fst (fmla_fv f))),
+    NoDup (map fst (fmla_fv (alpha_f_aux f l)))
+  )
+  .
+Proof.
+  revert t f. apply term_formula_ind; simpl; intros; 
+  try solve[repeat (constructor; auto)].
+  - apply nodup_map_big_union_alt; [apply string_dec | |].
+    + intros. rewrite map2_combine in H0.
+      rewrite in_map_iff in H0.
+      destruct H0 as [[t1 l2] [Hx Hinx]]; subst.
+      simpl.
+      rewrite in_combine_iff in Hinx; wf_tac.
+      destruct Hinx as [i [Hi Hx]].
+      specialize (Hx tm_d nil). inv Hx.
+      rewrite Forall_forall in H.
+      apply H; wf_tac.
+      * eapply disj_sublist. apply split_lens_disj.
+        apply Hfv. wf_tac.
+        apply sublist_map.
+        apply sublist_big_union. wf_tac.
+      * eapply disj_sublist. apply split_lens_disj.
+        apply Hbnd. wf_tac.
+        apply sublist_map.
+        apply sublist_concat_map. wf_tac.
+      * apply nodup_map_big_union_inv with(x:=(nth i l1 tm_d)) in Ht; wf_tac.
+        intros. apply tm_fv_nodup.
+    + intros x y t1 t2.
+      rewrite -> !in_map2_iff with(d1:=tm_d)(d2:=nil); wf_tac.
+      intros [i [Hi Ht1]] [j [Hj Ht2]]; subst. intros.
+      rewrite -> !alpha_t_aux_fv in H0, H1; wf_tac;
+      try solve [
+        eapply disj_sublist; [apply split_lens_disj; [apply Hfv |] |
+          apply sublist_map, sublist_big_union]; wf_tac
+      ];
+      try solve [
+        eapply disj_sublist; [apply split_lens_disj; [apply Hbnd |] |
+          apply sublist_map, sublist_concat_map]; wf_tac
+      ].
+      eapply nodup_map_big_union_inv_alt in Ht.
+      apply Ht. 4: apply H0. 4: apply H1. all: wf_tac.
+      intros; apply tm_fv_nodup.
+  - (*Tlet*)
+    destruct l; inversion Hlen; subst. simpl. inversion Hl; subst.
+    apply nodup_map_union_alt; wf_tac; [apply string_dec | | |].
+    + apply H; wf_tac.
+      * eapply disj_sublist. apply firstn_disj.
+        apply (disj_cons_inv Hfv). 
+        apply sublist_map. apply union_sublist_l.
+      * eapply disj_sublist. apply firstn_disj.
+        apply (disj_cons_inv Hbnd). apply incl_tl.
+        rewrite map_app. apply sublist_app_l.
+      * apply nodup_map_union_inv in Ht.
+        -- apply Ht.
+        -- apply tm_fv_nodup.
+        -- apply remove_nodup. apply tm_fv_nodup.
+    + rewrite -> map_remove with(eq_dec2:=string_dec).
+      2: {
+        intros.
+        (*Idea: every free var either thing subbed in or there
+          before, if there before, contradicts s*)
+        (*THis is provable*)
+        admit.
+      }
+      simpl. (*Need inv lemma for remove nodups*)
+Admitted.
+
+
+(*Question: can we prove alpha result?*)
+Require Import GenElts.
+(*Before doing this, prove that a_convert_t/f full gives tm_wf_strong
+  (move after once finish)*)
+Lemma a_convert_all_t_strong_wf t l:
+  NoDup (map fst (tm_fv t)) ->
+  tm_wf_strong (a_convert_all_t t l).
+Proof.
+  intros Hnodup.
+  unfold tm_wf_strong.
+  split_all.
+  - assert (disj (gen_strs (Datatypes.length (tm_bnd t)) (l ++ tm_bnd t ++ tm_fv t)%list)
+      (map fst (tm_bnd t) ++ map fst (tm_fv t))).
+    {
+      intros x [Hinx1 Hinx2].
+      apply gen_strs_notin' in Hinx1.
+      (*TODO*)
+      rewrite !map_cat in Hinx1.
+      rewrite !in_app_iff in Hinx1.
+      not_or Hinx.
+      rewrite !in_app_iff in Hinx2.
+      destruct Hinx2; contradiction.
+    }
+    apply alpha_aux_fv_NoDup; auto. apply Ftrue.
+    + apply gen_strs_nodup.
+    + rewrite gen_strs_length; auto.
+    + eapply disj_sublist. apply H. apply sublist_app_r. 
+    + eapply disj_sublist. apply H. apply sublist_app_l.
+  - apply a_convert_all_t_bnd_nodup.
+  - intros. intros [Hinfv Hinbnd].
+    apply a_convert_all_t_bnd_notin in Hinbnd.
+    destruct Hinbnd.
+    apply H. clear -Hinfv.
+    rewrite -> !in_map_iff in *.
+    destruct_all. exists x0. split; auto.
+    erewrite alpha_equiv_t_fv.
+    apply H0.
+    apply a_convert_all_t_equiv.
+Qed.
+   
+(*TODO: start with this, then go back to alpha lemma*)
+
+Section StrongWfRec.
+
+(*Plan
+  1. Prove if Nodup names of bnd, then NoDup names of bnd for all subterms/fmlas
+  2. Prove that all bnd in subterms/fmlas are in t
+  3. Use the above (plus fv lemma) to show that
+    no overlap in subterms (or else overlap in t)
+  4. Prove that if strong condition holds, no free variable dups in any
+    subterm
+  5. put together (no induction)
+  *)
+
+(*Want to show: if we have a term satisfying this condition,
+  then it satisfies it recursively*)
+  (*
+Lemma wf_strong_rec_holds t f:
+  (forall (Hwf: tm_wf_strong t), tm_wf_strong_rec t) /\
+  (forall (Hwf: fmla_wf_strong f), fmla_wf_strong_rec f).
+Proof.
+  unfold tm_wf_strong_rec, fmla_wf_strong_rec.
+  rewrite -> P_subterms_equiv, P_subfmlas_equiv. split.
+  - intros. split_all; auto. 3: rewrite Forall_forall; auto.
+    + unfold tm_wf_strong in *.
+      destruct_all.
+
+  
+  split; intros. unfold tm_wf_strong;
+  revert t f. unfold tm_wf_strong_rec, fmla_wf_strong_rec. 
+  apply term_formula_ind; simpl; intros.
+  - cbn. split; auto.
+  - cbn. split; auto.
+  - cbn. split; auto.
+    simpl_forall.
+    revert H. apply Forall_impl_in.
+    intros. apply H0.
+    clear -Hwf H.
+    unfold tm_wf_strong in *.
+    simpl in *. split_all.
+    + induction l1; simpl in *; try contradiction.
+      destruct H; subst.
+      * erewrite -> map_union  with(eq_dec2:=string_dec) in H0.
+
+
+    
+    rewrite Forall_forall; intros.
+    
+    simpl.
+
+*)
+
+Print tm_wf_strong_rec.
 
 
 (*TODO: 
